WIP

matching-logic/src/Theories/Definedness_ProofSystem.v
@@ -841,7 +841,7 @@ Definition dt_exgen_from_fp (ψ : Pattern) (gpi : ProofInfo) : coEVarSet :=
       apply Ex_gen with (x := x) in IHpf.
       3: { simpl. set_solver. }
       2: { apply pile_evs_svs_kt.
-        { set_solver. }
+        { clear -Hpf2. set_solver. }
         { set_solver. }
         { reflexivity. }
         { clear. set_solver. }
@@ -4445,6 +4445,1021 @@ Proof.
   mlSpec "mH1".
   mlExact "mH1".
 Defined.
+
+Lemma impl_ctx_impl_pos {Σ : Signature} Γ ctx ϕ ψ sz i :
+  well_formed ϕ ->
+  well_formed ψ ->
+  well_formed (pcPattern ctx) ->
+  size' (pcPattern ctx) <= sz ->
+  is_positive_context ctx ->
+  ProofInfoLe (ExGen := ⊤, SVSubst := ⊤, KT := true, FP := ∅) i ->
+  Γ ⊢i ϕ ---> ψ using i ->
+  Γ ⊢i (emplace ctx ϕ) ---> (emplace ctx ψ) using i
+  (*with
+  impl_ctx_impl_neg {Σ : Signature} Γ ctx ϕ ψ sz i :
+  well_formed ϕ ->
+  well_formed ψ ->
+  well_formed (pcPattern ctx) ->
+  size' (pcPattern ctx) <= sz ->
+  is_negative_context ctx ->
+  ProofInfoLe BasicReasoning i ->
+  Γ ⊢i ϕ ---> ψ using i ->
+  Γ ⊢i (emplace ctx ψ) ---> (emplace ctx ϕ) using i*).
+Proof.
+  all: intros wfϕ wfψ wfc Hsz Hc pile H.
+  {
+    (*clear impl_ctx_impl_pos.*)
+
+    unfold emplace.
+
+    destruct ctx as [cvar cpatt].
+    simpl in *.
+
+    generalize dependent cpatt.
+
+    induction sz.
+    {
+      destruct cpatt; simpl in *; lia.
+    }
+
+    intros cpatt wfc Hs Hp.
+    destruct cpatt. all: simpl in *.
+
+    (* trivial cases *)
+    2,5,7: aapply A_impl_A;[eapply pile_trans;[|apply pile];try_solve_pile;try_solve_pile|wf_auto2].
+    (* not well formed cases*)
+    2,3: cbv in wfc; discriminate wfc.
+
+    {
+      destruct decide.
+      { assumption. }
+      { gapply A_impl_A. eapply pile_trans;[|apply pile]; try_solve_pile. wf_auto2. }
+    }
+
+    + (*Check prf_equiv_congruence*)
+      pose proof (IH := IHsz (cpatt1 $ cpatt2)).
+      feed specialize IH.
+      { wf_auto2. }
+      { simpl. admit. }
+      {
+        unfold is_positive_context in Hp. simpl in Hp.
+        unfold is_positive_context. simpl. assumption.
+      }
+      simpl free_evar_subst in IH.
+      assumption.
+    + pose proof (IH := IHsz (cpatt1 ---> cpatt2)).
+      feed specialize IH.
+      { wf_auto2. }
+      { simpl. admit. }
+      {
+        unfold is_positive_context in Hp. simpl in Hp.
+        unfold is_positive_context. simpl. assumption.
+      }
+      simpl free_evar_subst in IH.
+      assumption.
+    + remember (evar_fresh_s ({[cvar]} ∪ free_evars cpatt ∪ free_evars ψ ∪ free_evars ϕ)) as x.
+      pose proof (IH := IHsz (evar_open x 0 cpatt)).
+      feed specialize IH.
+      { wf_auto2. }
+      { rewrite evar_open_size'. lia. }
+      {
+        unfold is_positive_context in Hp. simpl in Hp.
+        unfold is_positive_context. simpl. clear -Hp. admit. (*TODO: make a lemma*)
+      }
+      rewrite <- evar_quantify_evar_open with (n := 0) (phi := cpatt^[[evar:cvar↦ϕ]]) (x := x).
+      rewrite <- evar_quantify_evar_open with (n := 0) (phi := cpatt^[[evar:cvar↦ψ]]) (x := x).
+      apply ex_quan_monotone.
+      { eapply pile_trans;[|apply pile]. try_solve_pile. }
+      unfold evar_open.
+      unfold evar_open in IH.
+      Search (_^[[evar:_↦_]]^[evar:_↦_]). (*no lemma? write one?*)
+      admit.
+      {
+        subst x. 
+        eapply evar_is_fresh_in_richer'.
+        2: { apply set_evar_fresh_is_fresh'. }
+        pose proof (Hfree := free_evars_free_evar_subst cpatt ψ cvar).
+        clear -Hfree.
+        set_solver.
+      }
+      { wf_auto2. }
+      {
+        subst x. 
+        eapply evar_is_fresh_in_richer'.
+        2: { apply set_evar_fresh_is_fresh'. }
+        pose proof (Hfree := free_evars_free_evar_subst cpatt ϕ cvar).
+        clear -Hfree.
+        set_solver.
+      }
+      { wf_auto2. }
+
+    + remember (svar_fresh_s (free_svars cpatt ∪ free_svars ψ ∪ free_svars ϕ)) as X.
+      pose proof (IH := IHsz (svar_open X 0 cpatt)).
+      feed specialize IH.
+      { wf_auto2. }
+      { rewrite svar_open_size'. lia. }
+      {
+        unfold is_positive_context in Hp. simpl in Hp.
+        unfold is_positive_context. simpl. clear -Hp. admit.
+      }
+      rewrite <- svar_quantify_svar_open with (n := 0) (phi := cpatt^[[evar:cvar↦ϕ]]) (X := X).
+      rewrite <- svar_quantify_svar_open with (n := 0) (phi := cpatt^[[evar:cvar↦ψ]]) (X := X).
+      apply mu_monotone.
+      { eapply pile_trans;[|apply pile]. try_solve_pile. }
+      {
+        unfold is_positive_context in Hp. simpl in Hp. 
+        unfold well_formed in wfc. simpl in wfc.
+        destruct_and! wfc.
+        pose proof (Hneg := free_evar_subst_preserves_no_negative_occurrence cvar cpatt ϕ 0).
+        feed specialize Hneg.
+        { wf_auto2. }
+        { assumption. }
+        cbn in Hp.
+        apply positive_negative_occurrence_db_named.
+        { assumption. }
+        { Search (svar_has_negative_occurrence _ (_^[[evar:_↦_]])). admit. } (*TODO: write lemma*)
+      }
+      { admit. }
+      unfold svar_open.
+      unfold svar_open in IH.
+      rewrite <- free_evar_subst_bsvar_subst.
+      rewrite <- free_evar_subst_bsvar_subst.
+      apply IH.
+      { wf_auto2. }
+      { unfold evar_is_fresh_in. set_solver. }
+      { wf_auto2. }
+      { unfold evar_is_fresh_in. set_solver. }
+      {
+        clear -HeqX.
+        intro Hcontra.
+        pose proof (Hfree := free_svars_free_evar_subst cpatt cvar ψ).
+        assert (X ∉ free_svars cpatt /\ X ∉ free_svars ψ).
+        {
+          subst.
+          split.
+          unfold svar_fresh_s.
+          unfold elements.
+          subst. admit. (*!!!*)
+        }
+        set_solver.
+      }
+      { wf_auto2. }
+      { admit. }
+      { wf_auto2. }
+  }
+Admitted.
+
+Lemma and_ctx_and {Σ : Signature} {syntax : Syntax} Γ ctx ϕ ψ sz i :
+  well_formed ϕ ->
+  well_formed ψ ->
+  well_formed (pcPattern ctx) ->
+  size' (pcPattern ctx) <= sz ->
+  Γ ⊢i is_predicate_pattern ψ using i ->
+  mu_free (pcPattern ctx) ->
+  ProofInfoLe (ExGen := ∅, SVSubst := ∅, KT := false, FP := ∅) i ->
+  Γ ⊢i ψ and (emplace ctx ϕ) <---> ψ and (emplace ctx (ψ and ϕ)) using i.
+Proof.
+  intros wfm wfψ wfc Hs Hp mf pile.
+  unfold emplace.
+
+  destruct ctx as [cvar cpatt].
+  simpl in *.
+
+  generalize dependent cpatt.
+
+  induction sz.
+  {
+    destruct cpatt; simpl in *; lia.
+  }
+
+  intros cpatt wfc Hs Hm.
+  destruct cpatt. all: simpl in *.
+
+  (* trivial cases *)
+  2,5,7: apply pf_iff_split;[wf_auto2|wf_auto2|aapply A_impl_A|aapply A_impl_A];wf_auto2.
+  (* not well formed cases*)
+  2,3: cbv in wfc; discriminate wfc.
+
+  {
+    destruct decide.
+    {
+      apply pf_iff_split; wf_auto2.
+      toMLGoal. wf_auto2. mlIntro. mlDestructAnd "0". mlSplitAnd.
+      { mlExact "1". }
+      {
+        mlSplitAnd.
+        * mlExact "1".
+        * mlExact "2".
+      }
+      toMLGoal. wf_auto2. mlIntro. mlDestructAnd "0". mlDestructAnd "2". mlSplitAnd.
+      * mlExact "1".
+      * mlExact "3".
+    }
+    { apply pf_iff_split;[wf_auto2|wf_auto2|aapply A_impl_A|aapply A_impl_A];wf_auto2. }
+  }
+  
+  + admit.
+  + admit.
+  + admit.
+  + pose proof (IH := IHsz (mu , cpatt)).
+    feed specialize IH.
+    { wf_auto2. }
+    { simpl. admit. }
+    { congruence. }
+    { congruence. }
+Admitted.
+
+Lemma mu_and_predicate_propagation {Σ : Signature} {syntax : Syntax} i Γ ϕ ψ X :
+  well_formed (mu, ϕ) ->
+  well_formed ψ ->
+  svar_is_fresh_in X ϕ ->
+  svar_is_fresh_in X ψ ->
+  ProofInfoLe AnyReasoning i ->
+  Γ ⊢i is_predicate_pattern ψ using i ->
+  Γ ⊢i (mu, (ψ and ϕ)) <---> (ψ and (mu, ϕ)) using i.
+Proof.
+  intros wfm wfψ fϕ fψ pile Hp.
+  assert (Hnno : no_negative_occurrence_db_b 0 (ψ and ϕ) = true).
+  {
+    unfold well_formed in wfm. destruct_and! wfm.
+    unfold well_formed_positive in H. destruct_and! H.
+    clear -H1 wfψ.
+    Search no_negative_occurrence_db_b patt_and.
+    unfold patt_and.
+    unfold patt_not.
+    admit.
+  }
+  
+  apply pf_iff_split.
+  { wf_auto2. }
+  { wf_auto2. }
+  
+  (* Makes set_solver work later in the proof. *)
+  unfold svar_is_fresh_in in fϕ, fψ.
+  
+  {
+    toMLGoal.
+    { wf_auto2. }
+    mlIntro "H".
+    mlSplitAnd; fromMLGoal.
+    {
+      apply Knaster_tarski.
+      { eapply pile_trans;[|apply pile]. try_solve_pile. }
+      { wf_auto2. }
+      unfold instantiate.
+      rewrite -> well_formed_bsvar_subst with (k := 0).
+      2: auto.
+      2: wf_auto2; admit.
+      toMLGoal.
+      { wf_auto2. admit. }
+      mlIntro.
+      mlDestructAnd "0".
+      mlExact "1".
+    }
+    {
+      rewrite <- svar_quantify_svar_open with (n := 0) (phi := (ψ and ϕ)) (X := X).
+      rewrite <- svar_quantify_svar_open with (n := 0) (phi := ϕ) (X := X) at 2.
+      apply mu_monotone.
+      { eapply pile_trans;[|apply pile]. try_solve_pile. }
+      { wf_auto2. set_solver. }
+      { wf_auto2. }
+      {
+        unfold svar_open.
+        mlSimpl.
+        gapply pf_conj_elim_r.
+        { eapply pile_trans;[|apply pile]. try_solve_pile. }
+        { wf_auto2. }
+        { wf_auto2. }
+      }
+      { assumption. }
+      { wf_auto2. }
+      { set_solver. }
+      { wf_auto2. admit. }
+    }
+  }
+  
+  {
+    toMLGoal.
+    { wf_auto2. }
+    mlRewrite (useBasicReasoning i (@patt_and_comm Σ Γ ψ (mu , ϕ) wfψ wfm)) at 1.
+    2: { eapply pile_trans;[|apply pile]. try_solve_pile. }
+    fromMLGoal.
+    apply lhs_from_and.
+    { wf_auto2. }
+    { wf_auto2. }
+    { wf_auto2. }
+
+    apply Knaster_tarski.
+    { eapply pile_trans;[|apply pile]. try_solve_pile. }
+    { wf_auto2. }
+
+    apply lhs_to_and.
+    { wf_auto2. admit. admit. }
+    { wf_auto2. }
+    { wf_auto2. }
+    
+    toMLGoal.
+    { wf_auto2. admit. admit. }
+    assert (Htmp : is_true (well_formed (mu , ϕ) ^ [ψ ---> (mu , ψ and ϕ)])).
+    admit.
+    mlRewrite (useBasicReasoning i (@patt_and_comm Σ Γ ((mu , ϕ) ^ [ψ ---> (mu , ψ and ϕ)]) ψ Htmp wfψ)) at 1.
+    2: { eapply pile_trans;[|apply pile]. try_solve_pile. }
+    
+    mlIntro "H".
+    mlApplyMeta Pre_fixp.
+    unfold instantiate.
+    mlSimpl.
+    fromMLGoal.
+    rewrite -> well_formed_bsvar_subst with (φ := ψ) (k := 0).
+    2: auto.
+    2: wf_auto2.
+
+    remember (evar_fresh_s (free_evars ϕ)) as x.
+    pose proof (H := and_ctx_and Γ
+      {|
+        pcEvar := x;
+        pcPattern := ϕ^[svar:0↦patt_free_evar x];
+      |}
+      (ψ ---> (mu , ψ and ϕ))
+      (ψ)
+      40
+      i
+      ).
+    unfold emplace in H. simpl in H.
+    feed specialize H.
+    { wf_auto2. }
+    { wf_auto2. }
+    { wf_auto2. }
+    { admit. }
+    { assumption. }
+    { admit. }
+    { apply pile_basic_generic'. }
+
+    toMLGoal.
+    { wf_auto2. admit. admit. }
+    (*mlRewrite H at 1.
+
+    remember (evar_fresh_s (free_evars ϕ)) as x.
+    pose proof (H := impl_ctx_impl_pos Γ
+      {|
+        pcEvar := x;
+        pcPattern := ϕ^[svar:0↦patt_free_evar x];
+      |}
+      (ψ and (ψ ---> (mu , ψ and ϕ)))
+      (mu , ψ and ϕ)
+      40
+      i
+      ).
+    unfold emplace in H. simpl in H.
+    feed specialize H.
+    { wf_auto2. }
+    { wf_auto2. }
+    { wf_auto2. }
+    { admit. }
+    { unfold is_positive_context. simpl. admit. }
+    { eapply pile_trans;[|apply pile]. try_solve_pile. }
+    toMLGoal.
+    { wf_auto2. }
+    { mlIntro "H". mlDestructAnd "H". mlApply "1". mlExact "0". }
+    
+    unfold free_evar_subst in H. simpl in H.*)
+Admitted.
+
+Theorem deduction_theorem {Σ : Signature} {syntax : Syntax} Γ ϕ ψ
+  (gpi : ProofInfo)
+  (pf : Γ ∪ {[ ψ ]} ⊢i ϕ using gpi) :
+  well_formed ϕ ->
+  well_formed ψ ->
+  theory ⊆ Γ ->
+  pi_generalized_evars gpi ## (gset_to_coGset (free_evars ψ)) ->
+  pi_substituted_svars gpi ## (gset_to_coGset (free_svars ψ)) ->
+  Γ ⊢i ⌊ ψ ⌋ ---> ϕ
+  using AnyReasoning.
+Proof.
+  intros wfϕ wfψ HΓ HnoExGen HnoSvarSubst.
+  destruct pf as [pf Hpf]. simpl.
+  induction pf.
+  - (* hypothesis *)
+    rename axiom into axiom0.
+    (* We could use [apply elem_of_union in e; destruct e], but that would be analyzing Prop
+        when building Set, which is prohibited. *)
+    destruct (decide (axiom0 = ψ)).
+    + subst.
+      eapply useGenericReasoning.
+      2: {
+        apply total_phi_impl_phi; assumption.
+      }
+      {
+        apply pile_evs_svs_kt.
+        {
+          clear. set_solver.
+        }
+        {
+          clear. set_solver.
+        }
+        { reflexivity. }
+        { clear. set_solver. }
+      }
+
+    + assert (axiom0 ∈ Γ).
+      { clear -e n. set_solver. }
+      toMLGoal.
+      { wf_auto2. }
+      mlIntro. mlClear "0". fromMLGoal.
+      eapply useGenericReasoning.
+      2: apply (hypothesis Γ axiom0 i H).
+      apply pile_evs_svs_kt.
+      {
+        set_solver.
+      }
+      {
+        set_solver.
+      }
+      {
+        simpl. reflexivity.
+      }
+      { clear. set_solver. }
+  - (* P1 *)
+    toMLGoal.
+    { wf_auto2. }
+    do 3 mlIntro. mlExactn 1.
+  - (* P2 *)
+    toMLGoal.
+    { wf_auto2. }
+    mlIntro. mlClear "0". fromMLGoal.
+    useBasicReasoning.
+    apply P2; assumption.
+  - (* P3 *)
+    toMLGoal.
+    { wf_auto2. }
+    mlIntro. mlClear "0". fromMLGoal.
+    useBasicReasoning.
+    apply P3; assumption.
+  - (* Modus Ponens *)
+    assert (well_formed phi2).
+    { unfold well_formed, well_formed_closed in *. simpl in *.
+      destruct_and!. split_and!; auto.
+    }
+    assert (well_formed phi1).
+    {
+      clear -pf1. apply proved_impl_wf in pf1. exact pf1.
+    }
+
+    remember_constraint as i'.
+
+    destruct Hpf as [Hpf2 Hpf3 Hpf4].
+    simpl in Hpf2, Hpf3, Hpf4.
+    feed specialize IHpf1.
+    {
+      constructor; simpl.
+      { set_solver. }
+      { set_solver. }
+      { unfold implb in *.
+        destruct (uses_kt pf1) eqn:Hktpf1;[|reflexivity]. simpl in *.
+        exact Hpf4.
+      }
+      { clear -pwi_pf_fp. set_solver. }
+    }
+    { assumption. }
+    feed specialize IHpf2.
+    {
+      constructor; simpl.
+      { set_solver. }
+      { set_solver. }
+      { unfold implb in *.
+        destruct (uses_kt pf2) eqn:Hktpf2;[|reflexivity].
+        rewrite orb_comm in Hpf4. simpl in *.
+        exact Hpf4.
+      }
+      {
+        clear -pwi_pf_fp. set_solver.
+      }
+    }
+    { wf_auto2. }
+    
+    (*
+    (* simplify the constraint *)
+    unfold dt_exgen_from_fp. simpl.
+    rewrite map_app.
+    rewrite list_to_set_app_L.
+    simpl.
+    *)
+
+    (*
+    (* weaken the induction hypotheses so that their constraint
+        matches the constraint of the goal *)
+    apply useGenericReasoning with (i := i') in IHpf1.
+    2: {
+      subst i'.
+      apply pile_evs_svs_kt.
+      { clear. set_solver. }
+      { clear. set_solver. }
+      { reflexivity. }
+    }
+
+    apply useGenericReasoning with (i := i') in IHpf2.
+    2: {
+      subst i'.
+      apply pile_evs_svs_kt.
+      { clear. set_solver. }
+      { clear. set_solver. }
+      { reflexivity. }
+    }
+    *)
+
+    toMLGoal.
+    { wf_auto2. }
+    mlIntro.
+    mlAdd IHpf2.
+    mlAssert ((phi1 ---> phi2)).
+    { wf_auto2. }
+    { mlApply "1". mlExactn 1. }
+    mlApply "2".
+    mlAdd IHpf1.
+    mlApply "3".
+    mlExactn 2.
+  - (* Existential Quantifier *)
+    toMLGoal.
+    { wf_auto2. }
+    mlIntro. mlClear "0". fromMLGoal.
+    useBasicReasoning.
+    apply Ex_quan. wf_auto2.
+  - (* Existential Generalization *)
+    destruct Hpf as [Hpf2 Hpf3 Hpf4].
+    simpl in Hpf2, Hpf3, Hpf4.
+    (*
+    simpl in HnoExGen.
+    case_match;[congruence|]. *)
+    feed specialize IHpf.
+    {
+      constructor; simpl.
+      { clear -Hpf2. set_solver. }
+      { clear -Hpf3. set_solver. }
+      { apply Hpf4. }
+      { clear -pwi_pf_fp. set_solver. }
+    }
+    { wf_auto2. }
+
+    apply reorder_meta in IHpf.
+    2-4: wf_auto2.
+    apply Ex_gen with (x := x) in IHpf.
+    3: { simpl. set_solver. }
+    2: { apply pile_evs_svs_kt.
+      { set_solver. }
+      { set_solver. }
+      { reflexivity. }
+      { clear. set_solver. }
+    }
+    apply reorder_meta in IHpf.
+    2-4: wf_auto2.
+    exact IHpf.
+    
+  - (* Propagation of ⊥, left *)
+    toMLGoal.
+    { wf_auto2. }
+    mlIntro. mlClear "0". fromMLGoal.
+    useBasicReasoning.
+    apply Prop_bott_left; assumption.
+  - (* Propagation of ⊥, right *)
+    toMLGoal.
+    { wf_auto2. }
+    mlIntro. mlClear "0"; auto. fromMLGoal.
+    useBasicReasoning.
+    apply Prop_bott_right; assumption.
+  - (* Propagation of 'or', left *)
+    toMLGoal.
+    { wf_auto2. }
+    mlIntro. mlClear "0"; auto. fromMLGoal.
+    useBasicReasoning.
+    apply Prop_disj_left; assumption.
+  - (* Propagation of 'or', right *)
+    toMLGoal.
+    { wf_auto2. }
+    mlIntro. mlClear "0"; auto. fromMLGoal.
+    useBasicReasoning.
+    apply Prop_disj_right; assumption.
+  - (* Propagation of 'exists', left *)
+    toMLGoal.
+    { wf_auto2. }
+    mlIntro. mlClear "0"; auto. fromMLGoal.
+    useBasicReasoning.
+    apply Prop_ex_left; assumption.
+  - (* Propagation of 'exists', right *)
+    toMLGoal.
+    { wf_auto2. }
+    mlIntro. mlClear "0"; auto. fromMLGoal.
+    useBasicReasoning.
+    apply Prop_ex_right; assumption.
+  - (* Framing left *)
+    assert (well_formed (phi1)).
+    { unfold well_formed,well_formed_closed in *. simpl in *.
+      destruct_and!. split_and!; auto. }
+
+    assert (well_formed (phi2)).
+    { unfold well_formed,well_formed_closed in *. simpl in *.
+      destruct_and!. split_and!; auto. }
+
+    assert (well_formed (psi)).
+    { unfold well_formed,well_formed_closed in *. simpl in *.
+      destruct_and!. split_and!; auto. }
+    
+    assert (well_formed (phi1 ---> phi2)).
+    { unfold well_formed,well_formed_closed in *. simpl in *.
+      destruct_and!. split_and!; auto. }
+    destruct Hpf as [Hpf2 Hpf3 Hpf4].
+    simpl in Hpf2,Hpf3,Hpf4.
+    feed specialize IHpf.
+    {
+      constructor; simpl.
+      { set_solver. }
+      { set_solver. }
+      { apply Hpf4. }
+      { clear -pwi_pf_fp. set_solver. }
+    }
+    { wf_auto2. }
+
+    remember_constraint as i'.
+
+    (*
+    apply useGenericReasoning with (i0 := i') in IHpf.
+    2: {
+      subst i'.
+      apply pile_evs_svs_kt.
+      { clear. set_solver. }
+      { apply reflexivity. }
+      { reflexivity. }
+    }
+    *)
+    assert (S2: Γ ⊢i phi1 ---> (phi2 or ⌈ ! ψ ⌉) using i').
+    { toMLGoal.
+      { wf_auto2. }
+      mlAdd IHpf. mlIntro.
+      mlAdd (useBasicReasoning i' (A_or_notA Γ (⌈ ! ψ ⌉) ltac:(wf_auto2))).
+      mlDestructOr "0".
+      - mlRight. mlExact "3".
+      - mlLeft.
+        mlApply "4". mlExact "1".
+    }
+
+    assert (S3: Γ ⊢i (⌈ ! ψ ⌉ $ psi) ---> ⌈ ! ψ ⌉ using i').
+    {
+      replace (⌈ ! ψ ⌉ $ psi)
+        with (subst_ctx (ctx_app_l AC_patt_defined psi ltac:(assumption)) (! ψ))
+        by reflexivity.
+      subst i'.
+      gapply in_context_impl_defined; auto.
+      (*eapply useGenericReasoning. *)
+      (*2: apply in_context_impl_defined; auto.*)
+      apply pile_evs_svs_kt.
+      {
+        replace (free_evars (! ψ)) with (free_evars (ψ)).
+        2: {
+          simpl. set_solver.
+        }
+        simpl.
+        replace (free_evars psi ∪ (∅ ∪ ∅)) with (free_evars psi) by (clear; set_solver).
+        clear -pwi_pf_fp.
+        unfold dt_exgen_from_fp.
+        apply top_subseteq.
+      }
+      { clear. set_solver. }
+      { reflexivity. }
+      { clear. set_solver. }
+    }
+
+    assert (S4: Γ ⊢i (phi1 $ psi) ---> ((phi2 or ⌈ ! ψ ⌉) $ psi) using i').
+    { 
+      unshelve (eapply Framing_left).
+      { wf_auto2. } 2: exact S2.
+      subst i'. clear. try_solve_pile.
+    }
+
+    assert (S5: Γ ⊢i (phi1 $ psi) ---> ((phi2 $ psi) or (⌈ ! ψ ⌉ $ psi)) using i').
+    {
+      pose proof (Htmp := prf_prop_or_iff Γ (ctx_app_l box psi ltac:(assumption)) phi2 (⌈! ψ ⌉)).
+      feed specialize Htmp.
+      { wf_auto2. }
+      { wf_auto2. }
+      simpl in Htmp.
+      apply pf_iff_proj1 in Htmp.
+      3: wf_auto2.
+      2: wf_auto2.
+      subst i'.
+      eapply syllogism_meta.
+      5: {
+        gapply Htmp.
+        clear. try_solve_pile.
+      }
+      4: assumption.
+      all: wf_auto2.
+    }
+
+    assert (S6: Γ ⊢i ((phi2 $ psi) or (⌈ ! ψ ⌉ $ psi)) ---> ((phi2 $ psi) or (⌈ ! ψ ⌉)) using i').
+    {
+      toMLGoal.
+      { wf_auto2. }
+      mlIntro. mlAdd S3.
+      (* TODO we need a tactic for adding  something with stronger constraint. *)
+      mlAdd (useBasicReasoning i' (A_or_notA Γ (phi2 $ psi) ltac:(auto))).
+      mlDestructOr "2".
+      - mlLeft. mlExact "3".
+      - mlRight. mlApply "1". mlApply "0". mlExactn 0.
+    }
+
+    assert (S7: Γ ⊢i (phi1 $ psi) ---> ((phi2 $ psi)  or ⌈ ! ψ ⌉) using i').
+    {
+      toMLGoal.
+      { wf_auto2. }
+      mlAdd S5. mlAdd S6. mlIntro.
+      mlAssert (((phi2 $ psi) or (⌈ ! ψ ⌉ $ psi))).
+      { wf_auto2. }
+      { mlApply "0". mlExactn 2. }
+      mlDestructOr "3".
+      - mlLeft. mlExactn 3.
+      - mlApply "1". mlRight. mlExactn 3.
+    }
+
+    toMLGoal.
+    { wf_auto2. }
+    do 2 mlIntro. mlAdd S7.
+    mlAssert ((phi2 $ psi or ⌈ ! ψ ⌉)).
+    { wf_auto2. }
+    { mlApply "2". mlExactn 2. }
+    mlDestructOr "3".
+    + mlExactn 3.
+    + mlAssert ((phi2 $ psi or ⌈ ! ψ ⌉)).
+      { wf_auto2. }
+      { mlApply "2". mlExactn 2. }
+      mlAdd (useBasicReasoning i' (A_or_notA Γ (phi2 $ psi) ltac:(auto))).
+      mlDestructOr "4".
+      * mlExactn 0.
+      * mlAdd (useBasicReasoning i' (bot_elim Γ (phi2 $ psi) ltac:(auto))).
+        mlApply "4".
+        mlApply "0".
+        mlExactn 5.
+  - (* Framing right *)
+    assert (well_formed (phi1)).
+    { unfold well_formed,well_formed_closed in *. simpl in *.
+      destruct_and!. split_and!; auto. }
+
+    assert (well_formed (phi2)).
+    { unfold well_formed,well_formed_closed in *. simpl in *.
+      destruct_and!. split_and!; auto. }
+
+    assert (well_formed (psi)).
+    { unfold well_formed,well_formed_closed in *. simpl in *.
+      destruct_and!. split_and!; auto. }
+
+    assert (well_formed (phi1 ---> phi2)).
+    { unfold well_formed,well_formed_closed in *. simpl in *.
+      destruct_and!. split_and!; auto. }
+    simpl in HnoExGen. simpl in HnoSvarSubst.
+
+    destruct Hpf as [Hpf2 Hpf3 Hpf4].
+    simpl in Hpf2,Hpf3,Hpf4.
+    feed specialize IHpf.
+    {
+      constructor; simpl.
+      { set_solver. }
+      { set_solver. }
+      { apply Hpf4. }
+      { clear -pwi_pf_fp. set_solver. }
+    }
+    { wf_auto2. }
+
+
+    remember_constraint as i'.
+
+    (*
+    apply useGenericReasoning with (i := i') in IHpf.
+    2: {
+      subst i'.
+      apply pile_evs_svs_kt.
+      { clear. set_solver. }
+      { apply reflexivity. }
+      { reflexivity. }
+    }
+    *)
+    assert (S2: Γ ⊢i phi1 ---> (phi2 or ⌈ ! ψ ⌉) using i').
+    { toMLGoal.
+      { wf_auto2. }
+      mlAdd IHpf. mlIntro.
+      mlAdd (useBasicReasoning i' (A_or_notA Γ (⌈ ! ψ ⌉) ltac:(wf_auto2))).
+      mlDestructOr "2".
+      - mlRight. mlExactn 0.
+      - mlLeft.
+        mlAssert((phi1 ---> phi2)).
+        { wf_auto2. }
+        { mlApply "0". mlExactn 0. }
+        mlApply "2". mlExactn 2.
+    }
+
+    assert (S3: Γ ⊢i (psi $ ⌈ ! ψ ⌉) ---> ⌈ ! ψ ⌉ using i').
+    {
+      replace (psi $ ⌈ ! ψ ⌉)
+        with (subst_ctx (ctx_app_r psi AC_patt_defined ltac:(assumption)) (! ψ))
+        by reflexivity.
+        subst i'.
+        gapply in_context_impl_defined; auto.
+
+        apply pile_evs_svs_kt.
+        {
+          replace (free_evars (! ψ)) with (free_evars (ψ)).
+          2: {
+            simpl. set_solver.
+          }
+          simpl.
+          replace (free_evars psi ∪ (∅ ∪ ∅)) with (free_evars psi) by set_solver.
+
+          clear -pwi_pf_fp.
+          unfold dt_exgen_from_fp.
+          apply top_subseteq.
+        }
+        { clear. set_solver. }
+        { reflexivity. }
+        { clear. set_solver. }
+    }
+
+    assert (S4: Γ ⊢i (psi $ phi1) ---> (psi $ (phi2 or ⌈ ! ψ ⌉)) using i').
+    { 
+      (* TODO: have a variant of apply which automatically solves all wf constraints.
+          Like: unshelve (eapply H); try_wfauto
+      *)
+      unshelve (eapply Framing_right).
+      { wf_auto2. }
+      2: exact S2.
+      subst i'. try_solve_pile.
+    }
+
+    assert (S5: Γ ⊢i (psi $ phi1) ---> ((psi $ phi2) or (psi $ ⌈ ! ψ ⌉)) using i').
+    {
+      pose proof (Htmp := prf_prop_or_iff Γ (ctx_app_r psi box ltac:(assumption)) phi2 (⌈! ψ ⌉)).
+      feed specialize Htmp.
+      { wf_auto2. }
+      { wf_auto2. }
+      simpl in Htmp.
+      apply pf_iff_proj1 in Htmp.
+      2,3: wf_auto2.
+      subst i'.
+      eapply syllogism_meta.
+      5: gapply Htmp; try_solve_pile.
+      4: assumption.
+      all: wf_auto2.
+    }
+
+    assert (S6: Γ ⊢i ((psi $ phi2) or (psi $ ⌈ ! ψ ⌉)) ---> ((psi $ phi2) or (⌈ ! ψ ⌉)) using i').
+    {
+      toMLGoal.
+      { wf_auto2. }
+      mlIntro. mlAdd S3.
+      mlAdd (useBasicReasoning i' (A_or_notA Γ (psi $ phi2) ltac:(auto))).
+      mlDestructOr "2".
+      - mlLeft. mlExactn 0.
+      - mlRight. mlApply "1". mlApply "0". mlExactn 0.
+    }
+
+    assert (S7: Γ ⊢i (psi $ phi1) ---> ((psi $ phi2)  or ⌈ ! ψ ⌉) using i').
+    {
+      toMLGoal.
+      { wf_auto2. }
+      mlAdd S5. mlAdd S6. mlIntro.
+      mlAssert (((psi $ phi2) or (psi $ ⌈ ! ψ ⌉))).
+      { wf_auto2. }
+      { mlApply "0". mlExactn 2. }
+      mlDestructOr "3".
+      - mlLeft. mlExactn 3.
+      - mlApply "1". mlRight. mlExactn 3.
+    }
+
+    toMLGoal.
+    { wf_auto2. }
+    do 2 mlIntro. mlAdd S7.
+    mlAssert ((psi $ phi2 or ⌈ ! ψ ⌉)).
+    { wf_auto2. }
+    { mlApply "2". mlExactn 2. }
+    mlDestructOr "3".
+    + mlExactn 3.
+    + mlAssert ((psi $ phi2 or ⌈ ! ψ ⌉)).
+      { wf_auto2. }
+      { mlApply "2". mlExactn 2. }
+      mlAdd (useBasicReasoning i' (A_or_notA Γ (psi $ phi2) ltac:(auto))).
+      mlDestructOr "4".
+      * mlExactn 0.
+      * mlAdd (useBasicReasoning i' (bot_elim Γ (psi $ phi2) ltac:(auto))).
+        mlApply "4".
+        mlApply "0".
+        mlExactn 5.
+  - (* Set variable substitution *)
+    simpl in HnoExGen. simpl in HnoSvarSubst. simpl in IHpf.
+    destruct Hpf as [Hpf2 Hpf3 Hpf4].
+    simpl in Hpf2, Hpf3, Hpf4.
+    feed specialize IHpf.
+    {
+      constructor; simpl.
+      { exact Hpf2. }
+      { clear -Hpf3. set_solver. }
+      { exact Hpf4. }
+      { clear -pwi_pf_fp. set_solver. }
+    }
+    {
+      wf_auto2.
+    }
+    
+    remember_constraint as i'.
+
+    replace (⌊ ψ ⌋ ---> phi^[[svar: X ↦ psi]])
+      with ((⌊ ψ ⌋ ---> phi)^[[svar: X ↦ psi]]).
+    2: {  simpl.
+          rewrite [ψ^[[svar: X ↦ psi]]]free_svar_subst_fresh.
+          {
+            clear -HnoSvarSubst Hpf3. unfold svar_is_fresh_in. set_solver.
+          }
+          reflexivity.
+    }
+    apply Svar_subst.
+    3: {
+      apply IHpf.
+    }
+    {
+      subst i'.
+      apply pile_evs_svs_kt.
+      {
+        clear. set_solver.
+      }
+      {
+        clear -Hpf3. set_solver.
+      }
+      {
+          reflexivity.
+      }
+      { clear. set_solver. }
+    }
+    { wf_auto2. }
+
+  - (* Prefixpoint *)
+    toMLGoal.
+    { wf_auto2. }
+    mlIntro. mlClear "0". fromMLGoal.
+    apply useBasicReasoning.
+    apply Pre_fixp. wf_auto2.
+  - (* Knaster-Tarski *)
+    destruct Hpf as [Hpf2 Hpf3 Hpf4].
+    apply lhs_to_and.
+    1-3: wf_auto2.
+    remember_constraint as pi.
+
+    epose proof (Htmp := @mu_and_predicate_propagation _ _ pi Γ phi ⌊ ψ ⌋ ltac:(wf_auto2) ltac:(wf_auto2) _ _).
+    feed specialize Htmp.
+    { apply set_svar_fresh_is_fresh. }
+    { subst pi. simpl. try_solve_pile. }
+    { eapply (liftPi _ _ _ _ (@floor_is_predicate _ _ _ _ _ _)). }
+    toMLGoal.
+    wf_auto2.
+    mlIntro.
+    apply pf_iff_proj2 in Htmp.
+    mlApplyMeta Htmp in "0".
+    clear Htmp.
+    fromMLGoal.
+    apply Knaster_tarski.
+    1: subst pi; try_solve_pile.
+    all: wf_auto2.
+    1, 3: admit.
+
+    unfold instantiate.
+    mlSimpl.
+    apply lhs_from_and.
+
+    1-3: wf_auto2.
+    
+    rewrite -> well_formed_bsvar_subst with (k := 0).
+    simpl in IHpf.
+    apply IHpf.
+    constructor; try assumption.
+    {
+      clear -Hpf4.
+      destruct (uses_kt pf) eqn:H; rewrite H; simpl.
+      2: reflexivity.
+      simpl in Hpf4.
+      assumption.
+    }
+    { wf_auto2. }
+    { lia. }
+    { wf_auto2. } 
+
+
+  - (* Existence *)
+    toMLGoal.
+    { wf_auto2. }
+    mlIntro. mlClear "0". fromMLGoal.
+    apply useBasicReasoning.
+    apply Existence.
+  - (* Singleton *)
+    toMLGoal.
+    { wf_auto2. }
+    mlIntro. mlClear "0". fromMLGoal.
+    apply useBasicReasoning.
+    apply Singleton_ctx. wf_auto2.
+Admitted.
 
 Close Scope ml_scope.
 Close Scope string_scope.
